

Conditional Expectation

Stats 220A

Motivation: “best guess given information”

We have a probability space $(\Omega, \mathcal{F}, \mathbb{P})$ and a sub- σ -field $\mathcal{G} \subseteq \mathcal{F}$.

Think of \mathcal{G} as “information revealed” (e.g., what we have observed).

Goal: define $\mathbb{E}[X \mid \mathcal{G}]$ for $X \in L^1(\mathcal{F})$ so that

- ▶ it is \mathcal{G} -measurable (uses only information in \mathcal{G}),
- ▶ for every event $A \in \mathcal{G}$, it has the same average as X on A .

Definition (measure-theoretic)

Definition

Let $X \in L^1(\Omega, \mathcal{F}, \mathbb{P})$ and $\mathcal{G} \subseteq \mathcal{F}$. A random variable Y is a version of $\mathbb{E}[X \mid \mathcal{G}]$ if

1. Y is \mathcal{G} -measurable, and
2. for all $A \in \mathcal{G}$,

$$\int_A Y \, d\mathbb{P} = \int_A X \, d\mathbb{P}.$$

Notes:

- ▶ Defined up to a.s. equality.
- ▶ This is an *integral identity*, not a pointwise formula.

Two Fundamental Questions

We have defined $\mathbb{E}[X \mid \mathcal{G}]$ through an integral identity.

Natural questions:

- ▶ Does such a random variable Y actually exist?
- ▶ If it exists, is it unique?

We now show:

- ▶ Existence follows from the Radon–Nikodym theorem.
- ▶ Uniqueness holds up to almost sure equality.

Absolute Continuity and σ -Finiteness

Definition (Absolute Continuity)

Let ν and μ be measures on (Ω, \mathcal{F}) .

We say

$$\nu \ll \mu$$

if

$$\mu(A) = 0 \Rightarrow \nu(A) = 0 \quad \text{for all } A \in \mathcal{F}.$$

Definition (σ -finite measure)

A measure μ is called σ -finite if

$$\Omega = \bigcup_{n=1}^{\infty} A_n \quad \text{with} \quad \mu(A_n) < \infty.$$

Remark. Since $\mathbb{P}(\Omega) = 1 < \infty$, the probability measure \mathbb{P} is automatically σ -finite.

Radon–Nikodym Theorem

Radon–Nikodym Theorem.

Let ν and μ be σ -finite measures on (Ω, \mathcal{G}) . If $\nu \ll \mu$, then there exists a \mathcal{G} -measurable function f such that

$$\nu(A) = \int_A f \, d\mu \quad \forall A \in \mathcal{G}.$$

The function f is called the Radon–Nikodym derivative.

Existence: Case $X \geq 0$

Assume $X \geq 0$ and $X \in L^1$.

Define a set function ν on (Ω, \mathcal{G}) by

$$\nu(A) = \int_A X \, d\mathbb{P}, \quad A \in \mathcal{G}.$$

Step 1: ν is a measure on (Ω, \mathcal{G}) .

If (A_n) are disjoint in \mathcal{G} , then by monotone convergence,

$$\nu\left(\bigcup_n A_n\right) = \sum_n \nu(A_n).$$

Step 2: $\nu \ll \mathbb{P}|_{\mathcal{G}}$.

If $\mathbb{P}(A) = 0$, then $\nu(A) = 0$.

Notation. $\mathbb{P}|_{\mathcal{G}}$ denotes the restriction of \mathbb{P} to the σ -field \mathcal{G} , i.e.

$$\mathbb{P}|_{\mathcal{G}}(A) = \mathbb{P}(A), \quad A \in \mathcal{G}.$$

Apply Radon–Nikodym

Apply Radon–Nikodym with

$$\mu = \mathbb{P}|_{\mathcal{G}}, \quad \nu(A) = \int_A X \, d\mathbb{P}.$$

There exists a \mathcal{G} -measurable function $Y \geq 0$ such that

$$\nu(A) = \int_A Y \, d\mathbb{P} \quad \forall A \in \mathcal{G}.$$

Thus

$$\int_A X \, d\mathbb{P} = \int_A Y \, d\mathbb{P}.$$

Taking $A = \Omega$ shows Y is integrable.

So Y is a version of $\mathbb{E}[X \mid \mathcal{G}]$ for $X \geq 0$.

Existence: General Case

Let $X \in L^1$.

Write

$$X = X^+ - X^-,$$

where $X^+, X^- \geq 0$ and integrable.

Define

$$Y_1 = \mathbb{E}[X^+ \mid \mathcal{G}], \quad Y_2 = \mathbb{E}[X^- \mid \mathcal{G}].$$

Set

$$Y = Y_1 - Y_2.$$

Then for all $A \in \mathcal{G}$,

$$\int_A X \, d\mathbb{P} = \int_A Y \, d\mathbb{P}.$$

Thus $\mathbb{E}[X \mid \mathcal{G}]$ exists for all $X \in L^1$.

Uniqueness

Proposition

If Y_1, Y_2 satisfy the defining identity, then $Y_1 = Y_2$ a.s.

Proof.

Let $D = Y_1 - Y_2$.

For all $A \in \mathcal{G}$,

$$\int_A D d\mathbb{P} = 0.$$

Let $A_\varepsilon = \{D \geq \varepsilon\} \in \mathcal{G}$.

Then

$$0 = \int_{A_\varepsilon} D d\mathbb{P} \geq \varepsilon \mathbb{P}(A_\varepsilon).$$

Thus $\mathbb{P}(D > 0) = 0$ and similarly $\mathbb{P}(D < 0) = 0$.



First immediate consequence: law of total expectation

Proposition

For $X \in L^1(\mathcal{F})$,

$$\mathbb{E}[\mathbb{E}[X \mid \mathcal{G}]] = \mathbb{E}[X].$$

Proof.

Take $A = \Omega$ in the defining identity:

$$\int_{\Omega} \mathbb{E}[X \mid \mathcal{G}] d\mathbb{P} = \int_{\Omega} X d\mathbb{P}.$$



Interpretation: conditioning does not change the overall mean; it redistributes it across \mathcal{G} -events.

Example 1: conditioning on an event

Let $B \in \mathcal{F}$ with $0 < \mathbb{P}(B) < 1$ and $\mathcal{G} = \sigma(B) = \{\emptyset, B, B^c, \Omega\}$.

Proposition

For $X \in L^1$,

$$\mathbb{E}[X \mid \sigma(B)] = \frac{\mathbb{E}[X\mathbf{1}_B]}{\mathbb{P}(B)} \mathbf{1}_B + \frac{\mathbb{E}[X\mathbf{1}_{B^c}]}{\mathbb{P}(B^c)} \mathbf{1}_{B^c}.$$

Proof.

Let Y be the RHS. Then Y is $\sigma(B)$ -measurable (constant on B and B^c). Check the defining identity for $A = B$ and $A = B^c$:

$$\int_B Y \, d\mathbb{P} = \frac{\mathbb{E}[X\mathbf{1}_B]}{\mathbb{P}(B)} \mathbb{P}(B) = \mathbb{E}[X\mathbf{1}_B], \quad \int_{B^c} Y \, d\mathbb{P} = \mathbb{E}[X\mathbf{1}_{B^c}],$$

and the identity follows for all $A \in \sigma(B)$. □

Example 2: finite partition (general discrete information)

Let $\{A_1, \dots, A_n\}$ be a partition of Ω with $\mathbb{P}(A_i) > 0$ and $\mathcal{G} = \sigma(A_1, \dots, A_n)$.

Proposition

For $X \in L^1$,

$$\mathbb{E}[X \mid \mathcal{G}] = \sum_{i=1}^n \mathbb{E}[X \mid A_i] \mathbf{1}_{A_i} = \sum_{i=1}^n \frac{\mathbb{E}[X \mathbf{1}_{A_i}]}{\mathbb{P}(A_i)} \mathbf{1}_{A_i}.$$

Proof.

Same structure as the previous proof: define Y to be the RHS, note Y is \mathcal{G} -measurable, and verify the defining identity on generators $A = A_i$ (then extend by additivity over unions). □

Example 3: independence makes conditioning trivial

Proposition

If $X \in L^1$ is independent of \mathcal{G} , then

$$\mathbb{E}[X \mid \mathcal{G}] = \mathbb{E}[X] \quad a.s.$$

Proof.

Let $Y \equiv \mathbb{E}[X]$ (constant, hence \mathcal{G} -measurable). For any $A \in \mathcal{G}$, independence gives

$$\int_A X \, d\mathbb{P} = \mathbb{E}[X \mathbf{1}_A] = \mathbb{E}[X] \mathbb{E}[\mathbf{1}_A] = \mathbb{E}[X] \mathbb{P}(A) = \int_A Y \, d\mathbb{P}.$$

So Y satisfies the definition; uniqueness gives the claim. □

Example 4: conditioning on a random variable

Define

$$\mathbb{E}[X \mid Y] := \mathbb{E}[X \mid \sigma(Y)].$$

A key fact: $\mathbb{E}[X \mid Y]$ is a measurable function of Y .

Theorem (Doob–Dynkin lemma (informal statement))

If Z is $\sigma(Y)$ -measurable, then there exists a Borel measurable g such that $Z = g(Y)$ a.s.

So there exists g with

$$\mathbb{E}[X \mid Y] = g(Y) \quad \text{a.s.}$$

We will *use* this fact rather than prove it fully.

Concrete computation: independent sum

Let U, V be independent with $\mathbb{E}|V| < \infty$. Set $X = U + V$ and condition on U .

Proposition

$$\mathbb{E}[U + V \mid U] = U + \mathbb{E}[V] \quad a.s.$$

Proof.

Since U is $\sigma(U)$ -measurable,

$$\mathbb{E}[U + V \mid U] = \mathbb{E}[U \mid U] + \mathbb{E}[V \mid U] = U + \mathbb{E}[V],$$

where $\mathbb{E}[V \mid U] = \mathbb{E}[V]$ because V is independent of $\sigma(U)$. □

Concrete computation: bivariate normal (classic)

Let (X, Y) be jointly normal with means 0, variances 1, and correlation ρ .
Then:

$$\mathbb{E}[X \mid Y] = \rho Y, \quad \text{Var}(X \mid Y) = 1 - \rho^2.$$

Interpretation: conditioning on Y gives the best linear predictor, and for Gaussians it is the best predictor among all measurable functions.

Linearity and monotonicity

Proposition (Linearity)

If $X_1, X_2 \in L^1$ and $a, b \in \mathbb{R}$, then

$$\mathbb{E}[aX_1 + bX_2 \mid \mathcal{G}] = a\mathbb{E}[X_1 \mid \mathcal{G}] + b\mathbb{E}[X_2 \mid \mathcal{G}].$$

Proof.

Let $Y := a\mathbb{E}[X_1 \mid \mathcal{G}] + b\mathbb{E}[X_2 \mid \mathcal{G}]$. Then Y is \mathcal{G} -measurable. For any $A \in \mathcal{G}$,

$$\int_A Y \, d\mathbb{P} = a \int_A \mathbb{E}[X_1 \mid \mathcal{G}] \, d\mathbb{P} + b \int_A \mathbb{E}[X_2 \mid \mathcal{G}] \, d\mathbb{P} = a \int_A X_1 \, d\mathbb{P} + b \int_A X_2 \, d\mathbb{P} = \int_A (aX_1 + bX_2) \, d\mathbb{P}.$$

So Y satisfies the definition. □

Proposition (Monotonicity)

If $X \leq Y$ a.s., then $\mathbb{E}[X \mid \mathcal{G}] \leq \mathbb{E}[Y \mid \mathcal{G}]$ a.s.

Monotonicity (proof)

Proof.

Let $D := \mathbb{E}[X \mid \mathcal{G}] - \mathbb{E}[Y \mid \mathcal{G}]$ (which is \mathcal{G} -measurable). For $A := \{D > 0\} \in \mathcal{G}$ we have

$$\int_A D \, d\mathbb{P} = \int_A \mathbb{E}[X \mid \mathcal{G}] \, d\mathbb{P} - \int_A \mathbb{E}[Y \mid \mathcal{G}] \, d\mathbb{P} = \int_A X \, d\mathbb{P} - \int_A Y \, d\mathbb{P} \leq 0.$$

But on A , $D > 0$, hence $\int_A D \, d\mathbb{P} > 0$ unless $\mathbb{P}(A) = 0$. Therefore $\mathbb{P}(D > 0) = 0$, i.e. $D \leq 0$ a.s. □

Tower property

Proposition (Tower)

If $\mathcal{H} \subseteq \mathcal{G} \subseteq \mathcal{F}$ and $X \in L^1$, then

$$\mathbb{E}[\mathbb{E}[X \mid \mathcal{G}] \mid \mathcal{H}] = \mathbb{E}[X \mid \mathcal{H}] \quad a.s.$$

Proof.

Let $Y := \mathbb{E}[\mathbb{E}[X \mid \mathcal{G}] \mid \mathcal{H}]$. For any $A \in \mathcal{H}$,

$$\int_A Y \, d\mathbb{P} = \int_A \mathbb{E}[X \mid \mathcal{G}] \, d\mathbb{P} = \int_A X \, d\mathbb{P},$$

since $A \in \mathcal{H} \subseteq \mathcal{G}$. Thus Y satisfies the defining identity for conditioning on \mathcal{H} . □

Pull-out property: statement

We want the workhorse identity:

$$\mathbb{E}[ZX \mid \mathcal{G}] = Z \mathbb{E}[X \mid \mathcal{G}]$$

when Z is \mathcal{G} -measurable.

We prove it in steps:

1. $Z = \mathbf{1}_B$ with $B \in \mathcal{G}$
2. Z simple \mathcal{G} -measurable
3. $Z \geq 0$ \mathcal{G} -measurable (monotone limit)
4. integrable Z (positive/negative parts)

Pull-out property: proof (indicator and simple)

Proposition (Pull-out, bounded case)

If Z is bounded and \mathcal{G} -measurable and $X \in L^1$, then

$$\mathbb{E}[ZX \mid \mathcal{G}] = Z \mathbb{E}[X \mid \mathcal{G}] \quad \text{a.s.}$$

Proof.

Step 1: $Z = \mathbf{1}_B$, $B \in \mathcal{G}$. Let $A \in \mathcal{G}$. Then

$$\int_A \mathbf{1}_B \mathbb{E}[X \mid \mathcal{G}] d\mathbb{P} = \int_{A \cap B} \mathbb{E}[X \mid \mathcal{G}] d\mathbb{P} = \int_{A \cap B} X d\mathbb{P} = \int_A \mathbf{1}_B X d\mathbb{P}.$$

So $\mathbb{E}[\mathbf{1}_B X \mid \mathcal{G}] = \mathbf{1}_B \mathbb{E}[X \mid \mathcal{G}]$.

Step 2: $Z = \sum_{i=1}^m c_i \mathbf{1}_{B_i}$ simple \mathcal{G} -measurable. Use linearity and Step 1:

$$\mathbb{E}[ZX \mid \mathcal{G}] = \sum_i c_i \mathbb{E}[\mathbf{1}_{B_i} X \mid \mathcal{G}] = \sum_i c_i \mathbf{1}_{B_i} \mathbb{E}[X \mid \mathcal{G}] = Z \mathbb{E}[X \mid \mathcal{G}].$$

Pull-out property: proof (bounded via approximation)

Proof (continued).

Step 3: bounded \mathcal{G} -measurable Z . Approximate Z by simple functions Z_n with $Z_n \rightarrow Z$ a.s. and $|Z_n| \leq \|Z\|_\infty$.

Then $Z_n X \rightarrow ZX$ a.s. and $|Z_n X| \leq \|Z\|_\infty |X|$ which is integrable.

By dominated convergence,

$$\int_A Z_n X \, d\mathbb{P} \rightarrow \int_A ZX \, d\mathbb{P} \quad \text{for all } A \in \mathcal{G}.$$

Also $Z_n \mathbb{E}[X \mid \mathcal{G}] \rightarrow Z \mathbb{E}[X \mid \mathcal{G}]$ a.s. and is dominated by $\|Z\|_\infty |\mathbb{E}[X \mid \mathcal{G}]|$ with $\mathbb{E}|\mathbb{E}[X \mid \mathcal{G}]| \leq \mathbb{E}|X| < \infty$. So again dominated convergence gives

$$\int_A Z_n \mathbb{E}[X \mid \mathcal{G}] \, d\mathbb{P} \rightarrow \int_A Z \mathbb{E}[X \mid \mathcal{G}] \, d\mathbb{P}.$$

Since equality holds for each n , it holds in the limit. Uniqueness gives the result. □

L^2 orthogonality (full proof)

Assume $X \in L^2$. Let $Y = \mathbb{E}[X \mid \mathcal{G}]$.

Proposition (Orthogonality)

For every bounded \mathcal{G} -measurable Z ,

$$\mathbb{E}[(X - Y)Z] = 0.$$

Proof.

Since Z is \mathcal{G} -measurable and bounded, $(X - Y)Z \in L^1$. By the tower property and pull-out,

$$\mathbb{E}[(X - Y)Z] = \mathbb{E}[\mathbb{E}[(X - Y)Z \mid \mathcal{G}]] = \mathbb{E}[Z \mathbb{E}[X - Y \mid \mathcal{G}]] = \mathbb{E}[Z(Y - Y)] = 0.$$



Projection theorem in L^2

Theorem (Projection property)

Let $X \in L^2$ and $Y = \mathbb{E}[X \mid \mathcal{G}]$. Then for any $Z \in L^2(\mathcal{G})$,

$$\mathbb{E}[(X - Y)(Z - Y)] = 0 \quad \text{and} \quad \mathbb{E}[(X - Z)^2] = \mathbb{E}[(X - Y)^2] + \mathbb{E}[(Y - Z)^2].$$

In particular, Y minimizes $\mathbb{E}[(X - Z)^2]$ over $Z \in L^2(\mathcal{G})$.

Proof.

First, $(Z - Y) \in L^2(\mathcal{G})$, so approximate $(Z - Y)$ in L^2 by bounded \mathcal{G} -measurable functions and apply the orthogonality proposition (density argument). Then expand

$$(X - Z) = (X - Y) + (Y - Z)$$

and square:

$$(X - Z)^2 = (X - Y)^2 + (Y - Z)^2 + 2(X - Y)(Y - Z).$$

Take expectations; the cross term is zero by orthogonality.

Law of total variance

Theorem (Total variance)

If $X \in L^2$ then

$$\text{Var}(X) = \mathbb{E}[\text{Var}(X \mid \mathcal{G})] + \text{Var}(\mathbb{E}[X \mid \mathcal{G}]).$$

Proof.

Let $Y = \mathbb{E}[X \mid \mathcal{G}]$ and note $\mathbb{E}[Y] = \mathbb{E}[X]$.

Write

$$X - \mathbb{E}[X] = (X - Y) + (Y - \mathbb{E}[Y]).$$

Square and take expectations:

$$\text{Var}(X) = \mathbb{E}[(X - \mathbb{E}[X])^2] = \mathbb{E}[(X - Y)^2] + \mathbb{E}[(Y - \mathbb{E}[Y])^2] + 2\mathbb{E}[(X - Y)(Y - \mathbb{E}[Y])].$$

The cross term is 0 by orthogonality with $Z = (Y - \mathbb{E}[Y])$ (which is \mathcal{G} -measurable and in L^2). Finally, note $\mathbb{E}[(X - Y)^2] = \mathbb{E}[\mathbb{E}[(X - Y)^2 \mid \mathcal{G}]] = \mathbb{E}[\text{Var}(X \mid \mathcal{G})]$ by definition of conditional variance. □

Conditional Jensen

Theorem (Conditional Jensen)

If $\varphi : \mathbb{R} \rightarrow \mathbb{R}$ is convex and $X \in L^1$ with $\varphi(X) \in L^1$, then

$$\varphi(\mathbb{E}[X \mid \mathcal{G}]) \leq \mathbb{E}[\varphi(X) \mid \mathcal{G}] \quad a.s.$$

Proof idea (standard). A convex φ can be written as a supremum of affine functions:

$$\varphi(x) = \sup_{t \in T} \{a_t x + b_t\}.$$

Then for each t ,

$$a_t \mathbb{E}[X \mid \mathcal{G}] + b_t = \mathbb{E}[a_t X + b_t \mid \mathcal{G}] \leq \mathbb{E}[\varphi(X) \mid \mathcal{G}].$$

Taking \sup_t preserves \leq and yields Jensen.

L^p contraction

Theorem (L^p contraction)

For $p \geq 1$ and $X \in L^p$,

$$\|\mathbb{E}[X \mid \mathcal{G}]\|_p \leq \|X\|_p.$$

Proof.

Apply conditional Jensen to the convex function $\varphi(x) = |x|^p$:

$$|\mathbb{E}[X \mid \mathcal{G}]|^p \leq \mathbb{E}[|X|^p \mid \mathcal{G}] \quad \text{a.s.}$$

Take expectations and use total expectation:

$$\mathbb{E}|\mathbb{E}[X \mid \mathcal{G}]|^p \leq \mathbb{E} \mathbb{E}[|X|^p \mid \mathcal{G}] = \mathbb{E}|X|^p.$$



Worked example: conditioning reduces variance

Let $\mathcal{G} = \sigma(B)$ for an event B with $0 < \mathbb{P}(B) < 1$.

Then $\mathbb{E}[X \mid \mathcal{G}]$ is piecewise constant on B, B^c :

$$\mathbb{E}[X \mid \mathcal{G}] = \mathbb{E}[X \mid B]\mathbf{1}_B + \mathbb{E}[X \mid B^c]\mathbf{1}_{B^c}.$$

Total variance gives:

$$\text{Var}(X) = \mathbb{E}[\text{Var}(X \mid \mathcal{G})] + \text{Var}(\mathbb{E}[X \mid \mathcal{G}]).$$

So $\text{Var}(\mathbb{E}[X \mid \mathcal{G}])$ measures “how much of the variance is explained by knowing B ”.

Worked example: best L^2 predictor from a σ -field

Let $X \in L^2$ and consider predicting X using only information \mathcal{G} .

$$\hat{X} = g(\text{information in } \mathcal{G}) \iff \hat{X} \in L^2(\mathcal{G}).$$

Projection theorem says the unique minimizer of $\mathbb{E}[(X - \hat{X})^2]$ is

$$\hat{X}^* = \mathbb{E}[X \mid \mathcal{G}].$$

This is the mathematical meaning of “best mean-square prediction given \mathcal{G} ”.

Summary: what you should remember

- ▶ $\mathbb{E}[X \mid \mathcal{G}]$ is defined by an *integral identity* on all $A \in \mathcal{G}$.
- ▶ Existence comes from Radon–Nikodym; uniqueness holds a.s.
- ▶ Tower and pull-out are the workhorses.
- ▶ In L^2 , $\mathbb{E}[\cdot \mid \mathcal{G}]$ is an orthogonal projection.
- ▶ Total variance: $\text{Var}(X) = \mathbb{E}[\text{Var}(X \mid \mathcal{G})] + \text{Var}(\mathbb{E}[X \mid \mathcal{G}])$.
- ▶ Conditional Jensen $\Rightarrow L^p$ contraction.